testdata/cue/comprehensions/comprehension_body_pattern_local.cue
@@ -1,0 +1,6 @@
+out: {
+	for x in ["s"] {
+		a:        1
+		[string]: int
+	}
+}
